code/poly1305/Poly1305_64.fst
@@ -8,8 +8,101 @@ open FStar.HyperStack
 open FStar.Endianness
 open FStar.Buffer
 
-type uint8_p = Buffer.buffer Hacl.UInt8.t
+
 module U64  = FStar.UInt64
+module I = Hacl.Impl.Poly1305_64
+module S = Hacl.Spec.Poly1305_64
+
+(* Type Aliases *)
+type uint8_p = Buffer.buffer Hacl.UInt8.t
+type key = k:uint8_p{length k = 32}
+
+abstract type state = I.poly1305_state
+abstract type live_state (h:mem) (st:state) = I.live_st h st
+abstract type stable (h:mem) (st:state) = live_state h st /\ S.red_45 (as_seq h I.(st.h)) /\ S.red_44 (as_seq h I.(st.r))
+
+private let get_key (st:state) = I.MkState?.r st
+private let get_accumulator (st:state) = I.MkState?.h st
+
+#reset-options "--initial_fuel 0 --max_fuel 0 --z3rlimit 10"
+
+val alloc:
+  unit -> StackInline state
+    (requires (fun h -> True))
+    (ensures (fun h0 st h1 -> modifies_0 h0 h1 /\ live_state h1 st))
+let alloc () =
+  I.alloc()
+
+
+val init:
+  st:state ->
+  k:uint8_p{length k >= 16} ->
+  Stack unit
+    (requires (fun h -> live h k /\ live_state h st))
+    (ensures (fun h0 _ h1 -> modifies_2 (get_key st) (get_accumulator st) h0 h1 /\ stable h1 st))
+let init st k =
+  let _ = I.poly1305_init_ st (Buffer.sub k 0ul 16ul) in ()
+
+
+val update_block:
+  st:state ->
+  m:uint8_p{length m = 16} ->
+  Stack unit
+    (requires (fun h -> stable h st /\ live h m))
+    (ensures  (fun h0 updated_log h1 -> modifies_1 (get_accumulator st) h0 h1 /\ stable h1 st))
+let update_block st m =
+  let _ = I.poly1305_update (FStar.Ghost.hide (Seq.createEmpty)) st m in ()
+
+
+#reset-options "--initial_fuel 0 --max_fuel 0 --z3rlimit 100"
+
+val update:
+  st:state ->
+  m:uint8_p ->
+  len:FStar.UInt32.t{length m >= 16 * UInt32.v len} ->
+  Stack unit
+    (requires (fun h -> stable h st /\ live h m))
+    (ensures  (fun h0 updated_log h1 -> modifies_1 (get_accumulator st) h0 h1 /\ stable h1 st))
+let rec update st m len =
+  if FStar.UInt32.(len =^ 0ul) then ()
+  else 
+    let block = Buffer.sub m 0ul 16ul in
+    let m'    = Buffer.offset m 16ul  in
+    let len   = FStar.UInt32.(len -^ 1ul) in
+    let _ = update_block st block in
+    update st m' len
+
+  
+#reset-options "--initial_fuel 0 --max_fuel 0 --z3rlimit 10"
+
+module A = Hacl.Spec.Bignum.AddAndMultiply
+
+abstract type before_finish h st = A.(live_state h st /\ bounds (as_seq h (get_accumulator st)) p44 p44 p42)
+
+
+#reset-options "--initial_fuel 0 --max_fuel 0 --z3rlimit 100"
+
+val update_last:
+  st:state ->
+  m:uint8_p ->
+  len:UInt32.t{UInt32.v len < 16 /\ UInt32.v len <= length m} ->
+  Stack unit
+    (requires (fun h -> stable h st /\ live h m))
+    (ensures  (fun h0 _ h1 -> modifies_1 (get_accumulator st) h0 h1 /\ before_finish h1 st))
+let update_last st m len =
+  I.poly1305_update_last (FStar.Ghost.hide Seq.createEmpty) st (Buffer.sub m 0ul len) (Hacl.Cast.sint32_to_sint64 len)
+
+
+val finish:
+  st:state ->
+  mac:uint8_p{length mac = 16} ->
+  k:uint8_p{length k = 16} ->
+  Stack unit
+    (requires (fun h -> before_finish h st /\ live h mac /\ live h k))
+    (ensures (fun h0 _ h1 -> modifies_1 mac h0 h1))
+let finish st mac k =
+  I.poly1305_finish st mac k
+
 
 val crypto_onetimeauth:
   output:uint8_p{length output = 16} ->
